Delete crhs type and update proofs

compiler/backend/passes/proofs/pure_inline_cexpProofScript.sml
@@ -17,18 +17,14 @@ open pure_inline_relTheory pure_inline_cexpTheory pure_letrec_spec_cexpProofTheo
 
 val _ = new_theory "pure_inline_cexpProof";
 
-Definition crhs_to_rhs_def:
-  crhs_to_rhs (cExp e) = exp_of e
-End
-
 (* xs and m have the same elements *)
 Definition memory_inv_def:
   memory_inv xs m (ns:(mlstring,unit) map # num) ⇔
     { explode a | ∃e. lookup m a = SOME e } = set (MAP FST xs) ∧
     EVERY (λ(v,r). v ∈ set_of ns ∧ ∃e:'a cexp. avoid_set_ok ns e ∧ r = exp_of e) xs ∧
     ∀v e. (lookup m v = SOME e) ⇒
-          ∃e1. e = cExp (e1:'a cexp) ∧ cheap e1 ∧
-               MEM (explode v, (crhs_to_rhs e)) xs ∧
+          ∃e1. e = (e1:'a cexp) ∧ cheap e1 ∧
+               MEM (explode v, exp_of e) xs ∧
                avoid_set_ok ns e1 ∧
                NestedCase_free e1 ∧
                letrecs_distinct (exp_of e1) ∧
@@ -107,36 +103,20 @@ Theorem memory_inv_APPEND:
   letrecs_distinct (exp_of e1) ∧
   cexp_wf e1 ∧
   ¬MEM (explode v) (MAP FST xs) ⇒
-  memory_inv (xs ++ [(explode v,exp_of e1)]) (insert m v (cExp e1)) ns
+  memory_inv (xs ++ [(explode v,exp_of e1)]) (insert m v e1) ns
 Proof
   gvs [memory_inv_def]
-  \\ rw []
+  \\ disch_tac \\ fs []
+  \\ conj_tac
   >- (
     fs [EXTENSION,mlmapTheory.lookup_insert,AllCaseEqs()]
     \\ metis_tac []
   )
+  \\ conj_tac >- metis_tac []
   \\ gvs [mlmapTheory.lookup_insert,AllCaseEqs()]
-  \\ gvs [crhs_to_rhs_def,exp_of_def]
-  \\ first_x_assum $ irule_at Any \\ fs []
+  \\ strip_tac \\ gen_tac \\ disch_tac \\ fs []
+  \\ gvs [] \\ res_tac \\ fs []
 QED
-
-(*
-Theorem memory_inv_APPEND_Rec:
-  memory_inv xs m ∧
-  map_ok m ∧
-  ¬MEM (explode v) (MAP FST xs) ⇒
-  memory_inv (xs ++ [(explode v,Rec (exp_of e1))]) (insert m v (cRec e1))
-Proof
-  gvs [memory_inv_def]
-  \\ rw []
-  >- (
-    fs [EXTENSION,mlmapTheory.lookup_insert,AllCaseEqs()]
-    \\ metis_tac []
-  )
-  \\ gvs [mlmapTheory.lookup_insert,AllCaseEqs()]
-  \\ gvs [crhs_to_rhs_def,exp_of_def]
-QED
-*)
 
 Theorem DISJOINT_boundvars_Apps:
   ∀s e es.
@@ -561,8 +541,8 @@ Proof
   >~ [`Var _ _`] >- (
     gvs [inline_def]
     \\ Cases_on `lookup m v` \\ gvs [inline_rel_refl]
-    \\ Cases_on `x` \\ gvs [inline_rel_refl]
-    \\ Cases_on `is_Lam c` \\ gvs [memory_inv_def,inline_rel_refl,exp_of_def]
+    \\ gvs [inline_rel_refl]
+    \\ Cases_on `is_Lam x` \\ gvs [memory_inv_def,inline_rel_refl,exp_of_def]
     \\ Cases_on ‘cl = 0’ \\ gvs []
   )
   >~ [`App _ _ _`] >-
@@ -586,7 +566,7 @@ QED
 
 Definition mem_inv_def:
   mem_inv m ns =
-    ∀n v. lookup m n = SOME v ⇒ ∃e. avoid_set_ok ns e ∧ v = cExp e
+    ∀n v. lookup m n = SOME v ⇒ avoid_set_ok ns v
 End
 
 Theorem mem_inv_subset:
@@ -962,9 +942,9 @@ Proof
 QED
 
 Definition wf_mem_def:
-  wf_mem vars (m:(mlstring, 'a cexp_rhs) map) ⇔
+  wf_mem vars (m:(mlstring, 'a cexp) map) ⇔
     ∀n v. lookup m n = SOME v ⇒
-          ∃ce. v = cExp ce ∧ NestedCase_free ce ∧ avoid_set_ok vars ce ∧
+          ∃ce. v = ce ∧ NestedCase_free ce ∧ avoid_set_ok vars ce ∧
                cexp_wf ce ∧ letrecs_distinct (exp_of ce)
 End
 
@@ -1064,16 +1044,16 @@ Theorem LIST_REL_imp:
     LIST_REL
       (λce ce'.
          freevars (exp_of ce') ⊆ freevars (exp_of ce) ∪
-         {a | ∃n x. lookup m n = SOME (cExp x) ∧ a ∈ freevars (exp_of x)} ∧
+         {a | ∃n x. lookup m n = SOME x ∧ a ∈ freevars (exp_of x)} ∧
          cns_arities ce' ⊆ cns_arities ce ∪
-         {a | ∃n x. lookup m n = SOME (cExp x) ∧ a ∈ cns_arities x}) es es1
+         {a | ∃n x. lookup m n = SOME x ∧ a ∈ cns_arities x}) es es1
     ⇒
     BIGUNION (set (MAP freevars (MAP exp_of es1))) ⊆
     BIGUNION (set (MAP freevars (MAP exp_of es))) ∪
-    { a | ∃n x. lookup m n = SOME (cExp x) ∧ a ∈ freevars (exp_of x) } ∧
+    { a | ∃n x. lookup m n = SOME x ∧ a ∈ freevars (exp_of x) } ∧
     BIGUNION (set (MAP (λa. cns_arities a) es1)) ⊆
     BIGUNION (set (MAP (λa. cns_arities a) es)) ∪
-    { a | ∃n x. lookup m n = SOME (cExp x) ∧ a ∈ cns_arities x }
+    { a | ∃n x. lookup m n = SOME x ∧ a ∈ cns_arities x }
 Proof
   Induct \\ gvs [PULL_EXISTS]
   \\ rpt gen_tac \\ disch_tac \\ gvs []
@@ -1122,9 +1102,9 @@ fun wf_lemma () = inline_ind
        avoid_set_ok vars' ce' ∧
        freevars (exp_of ce') ⊆
        freevars (exp_of ce) ∪
-       { a | ∃n x. lookup m n = SOME (cExp x) ∧ a ∈ freevars (exp_of x) } ∧
+       { a | ∃n x. lookup m n = SOME x ∧ a ∈ freevars (exp_of x) } ∧
        cns_arities ce' ⊆ cns_arities ce ∪
-       { a | ∃n x. lookup m n = SOME (cExp x) ∧ a ∈ cns_arities x })’
+       { a | ∃n x. lookup m n = SOME x ∧ a ∈ cns_arities x })’
   |> Q.SPEC ‘λm vars cl h ce. ∀ce' vars'.
      inline_list m vars cl h ce = (ce',vars') ∧ wf_mem vars m ∧ map_ok m ∧
      EVERY (avoid_set_ok vars) ce ∧ EVERY NestedCase_free ce ∧ EVERY cexp_wf ce ∧
@@ -1135,9 +1115,9 @@ fun wf_lemma () = inline_ind
        EVERY letrecs_distinct (MAP exp_of ce') ∧
        LIST_REL (λce ce'.
          freevars (exp_of ce') ⊆ freevars (exp_of ce) ∪
-         { a | ∃n x. lookup m n = SOME (cExp x) ∧ a ∈ freevars (exp_of x) } ∧
+         { a | ∃n x. lookup m n = SOME x ∧ a ∈ freevars (exp_of x) } ∧
          cns_arities ce' ⊆ cns_arities ce ∪
-         { a | ∃n x. lookup m n = SOME (cExp x) ∧ a ∈ cns_arities x }) ce ce')’
+         { a | ∃n x. lookup m n = SOME x ∧ a ∈ cns_arities x }) ce ce')’
   |> CONV_RULE (DEPTH_CONV BETA_CONV);
 
 Theorem inline_wf_thm:
@@ -1224,8 +1204,8 @@ Proof
     \\ ‘wf_mem ns3 (heuristic_insert m h v e1) ∧
         avoid_set_ok ns3 e2 ∧
         map_ok (heuristic_insert m h v e1) ∧
-        ∀n y. lookup (heuristic_insert m h v e1) n = SOME (cExp y) ⇒
-              lookup m n = SOME (cExp y) ∨
+        ∀n y. lookup (heuristic_insert m h v e1) n = SOME y ⇒
+              lookup m n = SOME y ∨
               freevars (exp_of y) ⊆ freevars (exp_of e1) ∧
               cns_arities y ⊆ cns_arities e1’ by
       (irule_at Any wf_mem_subset >> rpt $ goal_assum $ drule_at Any >>
@@ -1269,8 +1249,8 @@ Proof
     \\ ‘wf_mem ns1 (heuristic_insert_Rec m h vbs) ∧
         map_ok (heuristic_insert_Rec m h vbs) ∧
         avoid_set_ok ns1 e ∧
-        ∀n y. lookup (heuristic_insert_Rec m h vbs) n = SOME (cExp y) ⇒
-              lookup m n = SOME (cExp y) ∨
+        ∀n y. lookup (heuristic_insert_Rec m h vbs) n = SOME y ⇒
+              lookup m n = SOME y ∨
               freevars (exp_of y) ⊆
               BIGUNION (set (MAP freevars (MAP (exp_of o SND) vbs))) ∧
               cns_arities y ⊆
@@ -1425,7 +1405,7 @@ Proof
                (MAP (λ(c,vs,e). freevars e DIFF set vs ∪ {explode v})
                   (MAP (λ(c,vs,x'). (explode c,MAP explode vs,exp_of x')) bs)))
              DELETE explode v ∪ freevars (exp_of e) ∪
-          {a | ∃n x. lookup m n = SOME (cExp x) ∧ a ∈ freevars (exp_of x)}’ by
+          {a | ∃n x. lookup m n = SOME x ∧ a ∈ freevars (exp_of x)}’ by
       (rpt gen_tac
        \\ qpat_x_assum ‘LIST_REL _ _ _’ mp_tac
        \\ qid_spec_tac ‘bs2’ \\ qid_spec_tac ‘bs’
@@ -1860,21 +1840,20 @@ Proof
     >- gvs [inline_rel_refl,exp_of_def]
     \\ gvs [inline_def]
     \\ Cases_on `lookup m v` \\ gvs [inline_rel_refl]
-    \\ Cases_on `x` \\ gvs [inline_rel_refl]
-    \\ Cases_on `is_Lam c` \\ gvs [memory_inv_def,inline_rel_refl,exp_of_def]
+    \\ Cases_on `is_Lam x` \\ gvs [memory_inv_def,inline_rel_refl,exp_of_def]
     \\ Cases_on ‘cl = 0’ \\ gvs []
     \\ first_assum drule \\ strip_tac \\ fs []
-    \\ gvs []
+    \\ fs []
     \\ irule_at Any inline_rel_Var
-    \\ fs [crhs_to_rhs_def]
+    \\ fs []
     \\ qpat_x_assum ‘MEM _ _’ $ irule_at Any
-    \\ qexists_tac ‘exp_of c’ \\ fs [exp_eq_refl]
-    \\ qsuff_tac ‘no_shadowing (exp_of c) ∧ boundvars (exp_of c) = {} ∧
-                  NestedCase_free c ∧
-                  letrecs_distinct (exp_of c) ∧ cexp_wf c’
+    \\ qexists_tac ‘exp_of x’ \\ fs [exp_eq_refl]
+    \\ qsuff_tac ‘no_shadowing (exp_of x) ∧ boundvars (exp_of x) = {} ∧
+                  NestedCase_free x ∧
+                  letrecs_distinct (exp_of x) ∧ cexp_wf x’
     >- (res_tac \\ fs [pre_def])
     \\ fs []
-    \\ Cases_on ‘c’ \\ gvs [cheap_def]
+    \\ Cases_on ‘x’ \\ gvs [cheap_def]
     \\ fs [exp_of_def,is_Lam_def,NULL_EQ]
   )
   >~ [`App _ _ _`] >- (
@@ -1916,33 +1895,18 @@ Proof
       \\ imp_res_tac inline_set_of \\ fs []
       \\ irule_at Any avoid_set_ok_subset \\ fs []
       \\ qexists_tac ‘ns’ \\ fs []
-      >-
-       (conj_tac \\ rw []
-        >- (gvs [SUBSET_DEF] \\ metis_tac [])
-        \\ last_x_assum drule
-        \\ metis_tac [avoid_set_ok_subset])
+      \\ conj_tac
+      >- (rw [] \\ gvs [SUBSET_DEF] \\ metis_tac [])
+      \\ conj_tac
+      >- (rw [] \\ last_x_assum drule
+          >- (gvs [SUBSET_DEF] \\ metis_tac [])
+          \\ metis_tac [avoid_set_ok_subset])
+      \\ rw []
+      \\ last_x_assum drule
+      \\ metis_tac [avoid_set_ok_subset]
     )
     \\ gvs []
     \\ rename [‘lookup m x = SOME aa’]
-    \\ reverse $ Cases_on `aa`
-    >- (
-      gvs [exp_of_def,SF ETA_ss]
-      \\ irule inline_rel_Apps
-      \\ fs [LIST_REL_MAP,o_DEF]
-      \\ last_x_assum $ irule_at Any
-      \\ last_x_assum $ irule_at Any
-      \\ gvs [memory_inv_def,DISJOINT_SYM]
-      \\ fs [EVERY_MAP,DISJOINT_SYM,cexp_wf_def]
-      \\ fs [EVERY_MEM,pure_expTheory.letrecs_distinct_def]
-      \\ imp_res_tac avoid_set_ok_imp_vars_ok \\ fs []
-      \\ imp_res_tac inline_set_of \\ fs []
-      \\ irule_at Any avoid_set_ok_subset \\ fs []
-      \\ qexists_tac ‘ns’ \\ fs []
-      \\ rw [] \\ first_x_assum drule
-      \\ strip_tac \\ gvs []
-      \\ irule_at Any avoid_set_ok_subset \\ fs []
-      \\ metis_tac []
-    )
     \\ gvs []
     \\ rpt (pairarg_tac \\ gvs [])
     \\ rename [`freshen_cexp _ _ = (q_fresh, r_fresh)`]
@@ -1957,6 +1921,7 @@ Proof
       \\ irule_at Any inline_rel_refl
       \\ fs [EVERY_MAP,DISJOINT_SYM,cexp_wf_def]
       \\ fs [EVERY_MEM,pure_expTheory.letrecs_distinct_def]
+      \\ metis_tac []
     )
     \\ gvs []
     \\ rename [`inline _ _ _ _ _ = (q_inline, r_inline)`]
@@ -1971,10 +1936,11 @@ Proof
       \\ irule_at Any inline_rel_refl
       \\ fs [EVERY_MAP,DISJOINT_SYM,cexp_wf_def]
       \\ fs [EVERY_MEM,pure_expTheory.letrecs_distinct_def]
+      \\ metis_tac []
     )
     \\ gvs []
     \\ Cases_on ‘e’ \\ gvs [get_Var_name_def,exp_of_def]
-    \\ rename [‘lookup m v = SOME (cExp c)’]
+    \\ rename [‘lookup m v = SOME c’]
     \\ first_x_assum drule
     \\ impl_tac >- fs [boundvars_Apps,EVERY_MEM,MEM_MAP,PULL_EXISTS,cexp_wf_def]
     \\ strip_tac
@@ -1988,7 +1954,7 @@ Proof
     \\ irule_at (Pos hd) inline_rel_Apps
     \\ irule_at (Pos hd) inline_rel_VarSimp
     \\ ‘MEM (explode v,exp_of c) xs’ by
-          (fs [memory_inv_def] \\ res_tac  \\ fs [crhs_to_rhs_def])
+          (fs [memory_inv_def] \\ res_tac  \\ fs [])
     \\ pop_assum $ irule_at Any
     \\ qexists_tac ‘MAP exp_of es1’
     \\ gvs [LIST_REL_MAP,pre_def]
@@ -2149,7 +2115,7 @@ Proof
     \\ irule inline_rel_App
     \\ reverse $ conj_tac
     >- (
-      last_x_assum irule
+      last_x_assum irule \\ fs []
       \\ fs [DISJOINT_SYM,memory_inv_def,cexp_wf_def]
     )
     \\ irule inline_rel_Lam
@@ -2426,6 +2392,7 @@ Proof
      (first_x_assum irule \\ fs []
       \\ gvs [cexp_wf_def,pure_expTheory.letrecs_distinct_def]
       \\ simp [DISJOINT_SYM]
+      \\ gvs [SF SFY_ss]
       \\ first_x_assum (fn th => mp_tac th \\ match_mp_tac avoid_set_ok_subset_exp)
       \\ gvs [allvars_def,exp_of_def]
       \\ simp [SUBSET_DEF])
